coq/src/HacspecIntegerDefinitions.v
@@ -1,0 +1,91 @@
+From Coq Require Import ZArith List.
+
+Inductive ints := U8
+             | U16
+             | U32
+             | U64
+             | U128.
+
+Definition wordsize {i} :=
+  match i with
+  | U8 => 8
+  | U16 => 16
+  | U32 => 32
+  | U64 => 64
+  | U128 => 128
+  end.
+Definition modulus {i : ints} : Z := two_power_nat (@wordsize i).
+Definition max_unsigned {i : ints} : Z := @modulus i - 1.
+
+Class WS (T : Type) : Type := {
+    translate : ints -> T ;
+    ws_wordsize : T -> nat ;
+    wordsize_eq : forall (i : ints), ws_wordsize (translate i) = @wordsize i ;
+
+    ws_modulus : T -> Z ;
+    modulus_eq : forall (i : ints), ws_modulus (translate i) = @modulus i ;
+
+    ws_max_unsigned : T -> Z ;
+    max_unsigned_eq : forall (i : ints), ws_max_unsigned (translate i) = @max_unsigned i ;
+  }.
+
+Class Integer (i : ints) {word_type} `{ws : WS word_type} :=
+  {
+    IntType : word_type -> Type ;
+    T : Type := IntType (translate i) ;
+    repr : Z -> T ;
+    unsigned : T -> Z ;
+    signed : T -> Z ;
+
+    rotate_left : forall (s u : T), T ;
+    rotate_right : forall (s u : T), T ;
+
+    add_int : forall (s u : T), T ;
+    sub_int : forall (s u : T), T ;
+    neg_int : forall (s : T), T  ;
+    mul_int : forall (s u : T), T  ;
+    divs_int : forall (s u : T), T  ;
+    mods_int : forall (s u : T), T  ;
+    xor_int : forall (s u : T), T ;
+    and_int : forall (s u : T), T ;
+    or_int : forall (s u : T), T ;
+
+    not : forall (s : T), T  ;
+    
+    eq_int : forall (s u : T), bool ;
+    lt_int : forall (s u : T), bool ;
+
+    shl_int : forall (s u : T), T ;
+    shr_int : forall (s u : T), T ;
+
+    zero : T ;
+    one : T ;
+
+    unsigned_repr : forall z, (0 <= z <= @max_unsigned i)%Z -> unsigned (repr z) = z ;
+    repr_unsigned : forall x, repr (unsigned x) = x ;
+    unsigned_range : forall x, (0 <= unsigned x < @modulus i)%Z ;
+
+    add_unsigned : forall x y, add_int x y = repr (unsigned x + unsigned y) ;
+    add_commut : forall x y , add_int x y = add_int y x ;
+    add_assoc: forall x y z, add_int (add_int x y) z = add_int x (add_int y z) ;
+
+    zero_is_repr_zero : repr (0%Z) = zero ;
+    add_zero_l : forall n, add_int zero n = n ;
+
+    unsigned_one : unsigned one = 1%Z ;
+
+    eq_leibniz_int : forall x y, eq_int x y = true <-> x = y ;
+  }.
+Definition IntegerType `(Integer) : Type := T.
+
+Global Infix "%%" := Z.rem (at level 40, left associativity) : Z_scope.
+Global Infix ".+" := add_int (at level 77) : hacspec_scope.
+Global Infix ".-" := sub_int (at level 77) : hacspec_scope.
+Global Notation "-" := neg_int (at level 77) : hacspec_scope.
+Global Infix ".*" := mul_int (at level 77) : hacspec_scope.
+Global Infix "./" := divs_int (at level 77) : hacspec_scope.
+Global Infix ".%" := mods_int (at level 77) : hacspec_scope.
+Global Infix ".^" := xor_int (at level 77) : hacspec_scope.
+Global Infix ".&" := and_int (at level 77) : hacspec_scope.
+Global Infix ".|" := or_int (at level 77) : hacspec_scope.
+Global Infix "==" := eq_int (at level 32) : hacspec_scope.
